p256: wip: clean up Hacl.Impl.P256.Point

code/ecdsap256/Hacl.Impl.P256.Point.fst
@@ -50,51 +50,7 @@ let make_point_at_inf p =
 let copy_point p res = copy res p
 
 
-(* https://crypto.stackexchange.com/questions/43869/point-at-infinity-and-error-handling*)
-val lemma_pointAtInfInDomain: x: nat -> y: nat -> z: nat {z < S.prime} ->
-  Lemma (S.isPointAtInfinity (x, y, z) == S.isPointAtInfinity ((fromDomain_ x), (fromDomain_ y), (fromDomain_ z)))
-
-let lemma_pointAtInfInDomain x y z =
-  assert (if S.isPointAtInfinity (x, y, z) then z == 0 else z <> 0);
-  assert_norm (S.modp_inv2 (pow2 256) % S.prime <> 0);
-  lemmaFromDomain z;
-  assert (fromDomain_ z == (z * S.modp_inv2 (pow2 256) % S.prime));
-  assert_norm (0 * S.modp_inv2 (pow2 256) % S.prime == 0);
-  lemma_multiplication_not_mod_prime z;
-  assert (if z = 0 then z * S.modp_inv2 (pow2 256) % S.prime == 0
-                   else fromDomain_ z <> 0)
-
-
-let isPointAtInfinityPrivate p =
-  let h0 = ST.get() in
-  let z0 = index p (size 8) in
-  let z1 = index p (size 9) in
-  let z2 = index p (size 10) in
-  let z3 = index p (size 11) in
-  let z0_zero = eq_mask z0 (u64 0) in
-  let z1_zero = eq_mask z1 (u64 0) in
-  let z2_zero = eq_mask z2 (u64 0) in
-  let z3_zero = eq_mask z3 (u64 0) in
-     eq_mask_lemma z0 (u64 0);
-     eq_mask_lemma z1 (u64 0);
-     eq_mask_lemma z2 (u64 0);
-     eq_mask_lemma z3 (u64 0);
-  let r = logand(logand z0_zero z1_zero) (logand z2_zero z3_zero) in
-    lemma_pointAtInfInDomain (as_nat h0 (gsub p (size 0) (size 4))) (as_nat h0 (gsub p (size 4) (size 4))) (as_nat h0 (gsub p (size 8) (size 4)));
-  r
-
-
-let isPointAtInfinityPublic p =
-  let z0 = index p (size 8) in
-  let z1 = index p (size 9) in
-  let z2 = index p (size 10) in
-  let z3 = index p (size 11) in
-  let z0_zero = eq_0_u64 z0 in
-  let z1_zero = eq_0_u64 z1 in
-  let z2_zero = eq_0_u64 z2 in
-  let z3_zero = eq_0_u64 z3 in
-  z0_zero && z1_zero && z2_zero && z3_zero
-
+///  Point conversion between Montgomery and Regular representations
 
 [@CInline]
 let point_to_mont p res =
@@ -126,46 +82,130 @@ let point_from_mont p res =
   fromDomain pz rz
 
 
+///  check if a point is a point-at-infinity
+
+(* https://crypto.stackexchange.com/questions/43869/point-at-infinity-and-error-handling*)
+val lemma_mont_is_point_at_inf: p:S.point_nat{let (_, _, z) = p in z < S.prime} ->
+  Lemma (S.isPointAtInfinity p == S.isPointAtInfinity (SM.fromDomainPoint p))
+
+let lemma_mont_is_point_at_inf p =
+  let px, py, pz = p in
+  assert (if S.isPointAtInfinity p then pz == 0 else pz <> 0);
+  assert (SM.fromDomain_ pz == pz * SM.mont_R_inv % S.prime);
+  assert_norm (SM.mont_R_inv % S.prime <> 0);
+  assert_norm (0 * SM.mont_R_inv % S.prime == 0);
+  lemma_multiplication_not_mod_prime pz;
+  assert (if pz = 0 then SM.fromDomain_ pz == 0 else SM.fromDomain_ pz <> 0)
+
+
+[@CInline]
+let is_point_at_inf p =
+  let h0 = ST.get () in
+  lemma_mont_is_point_at_inf (as_point_nat (as_seq h0 p));
+  let pz = getz p in
+  bn_is_zero_mask4 pz
+
+
+[@CInline]
+let is_point_at_inf_vartime p =
+  let pz = getz p in
+  bn_is_zero_vartime4 pz
+
+
+///  Point conversion between Jacobian and Affine coordinates representations
+
 inline_for_extraction noextract
-val normalisation_update: z2x: felem -> z3y: felem ->p: point ->  resultPoint: point -> Stack unit
-  (requires fun h -> live h z2x /\ live h z3y /\ live h resultPoint /\ live h p /\
-    as_nat h z2x < S.prime /\ as_nat h z3y < S.prime /\
-    as_nat h (gsub p (size 8) (size 4)) < S.prime /\
-    disjoint z2x z3y /\ disjoint z2x resultPoint /\ disjoint z3y resultPoint)
-  (ensures fun h0 _ h1 -> modifies (loc resultPoint) h0 h1 /\
-    (
-      let x0 = as_nat h0 (gsub p (size 0) (size 4)) in
-      let y0 = as_nat h0 (gsub p (size 4) (size 4)) in
-      let z0 = as_nat h0 (gsub p (size 8) (size 4)) in
+val norm_jacob_point_z: p:point -> res:felem -> Stack unit
+  (requires fun h ->
+    live h res /\ live h p /\ disjoint p res /\
+    point_z_as_nat h p < S.prime)
+  (ensures fun h0 _ h1 -> modifies (loc res) h0 h1 /\
+    (let _, _, rz = S.norm_jacob_point (SM.fromDomainPoint (as_point_nat (as_seq h0 p))) in
+    as_nat h1 res == rz))
 
-      let x1 = as_nat h1 (gsub resultPoint (size 0) (size 4)) in
-      let y1 = as_nat h1 (gsub resultPoint (size 4) (size 4)) in
-      let z1 = as_nat h1 (gsub resultPoint (size 8) (size 4)) in
+let norm_jacob_point_z p res =
+  push_frame ();
+  let fresero = create (size 4) (u64 0) in
+  let bit = is_point_at_inf p in
 
-      x1 == fromDomain_(as_nat h0 z2x) /\ y1 == fromDomain_(as_nat h0 z3y)  /\
-      (
-	if Spec.P256.isPointAtInfinity (fromDomain_ x0, fromDomain_ y0, fromDomain_ z0) then  z1 == 0 else z1 == 1
-      ))
-  )
+  bn_set_one4 res;
+  bn_copy_conditional4 res fresero bit;
+  pop_frame ()
 
 
-let normalisation_update z2x z3y p resultPoint =
-  push_frame();
-    let zeroBuffer = create (size 4) (u64 0) in
+[@CInline]
+let norm_jacob_point_x p res =
+  let px = getx p in
+  let pz = getz p in
 
-  let resultX = sub resultPoint (size 0) (size 4) in
-  let resultY = sub resultPoint (size 4) (size 4) in
-  let resultZ = sub resultPoint (size 8) (size 4) in
-    let h0 = ST.get() in
-  let bit = isPointAtInfinityPrivate p in
-  fromDomain z2x resultX;
-  fromDomain z3y resultY;
-  bn_set_one4 resultZ;
-    let h1 = ST.get() in
-  bn_copy_conditional4 resultZ zeroBuffer bit;
-    let h2 = ST.get() in
-  pop_frame()
+  let h0 = ST.get () in
+  fsqr pz res;       // rx = pz * pz
+  let h1 = ST.get () in
+  assert (fmont_as_nat h1 res == S.fmul (fmont_as_nat h0 pz) (fmont_as_nat h0 pz));
+  finv res res;       // rx = finv rx
+  let h2 = ST.get () in
+  assert (fmont_as_nat h2 res == S.finv (fmont_as_nat h1 res));
+  fmul px res res;    // rx = px * rx
+  let h3 = ST.get () in
+  assert (fmont_as_nat h3 res == S.fmul (fmont_as_nat h0 px) (fmont_as_nat h2 res));
+  fromDomain res res;
+  let h4 = ST.get () in
+  assert (as_nat h4 res == fmont_as_nat h3 res)
 
+
+// TODO: rm
+inline_for_extraction noextract
+val norm_jacob_point_y: p:point -> res:felem -> Stack unit
+  (requires fun h ->
+    live h res /\ live h p /\ disjoint p res /\
+    point_inv (as_seq h p))
+  (ensures fun h0 _ h1 -> modifies (loc res) h0 h1 /\
+    (let _, ry, _ = S.norm_jacob_point (SM.fromDomainPoint (as_point_nat (as_seq h0 p))) in
+    as_nat h1 res == ry))
+
+let norm_jacob_point_y p res =
+  let py = gety p in
+  let pz = getz p in
+
+  let h0 = ST.get () in
+  fcube pz res;       // ry = pz * pz * pz
+  let h1 = ST.get () in
+  finv res res;       // ry = finv ry
+  let h2 = ST.get () in
+  assert (fmont_as_nat h2 res == S.finv (fmont_as_nat h1 res));
+  fmul py res res;    // ry = px * ry
+  let h3 = ST.get () in
+  assert (fmont_as_nat h3 res == S.fmul (fmont_as_nat h0 py) (fmont_as_nat h2 res));
+  fromDomain res res;
+  let h4 = ST.get () in
+  assert (as_nat h4 res == fmont_as_nat h3 res)
+
+
+[@CInline]
+let norm_jacob_point p res =
+  push_frame ();
+  let tmp = create 12ul (u64 0) in
+  let tx = getx tmp in
+  let ty = gety tmp in
+  let tz = getz tmp in
+  norm_jacob_point_x p tx;
+  norm_jacob_point_y p ty;
+  norm_jacob_point_z p tz;
+  copy_point tmp res;
+  pop_frame ()
+
+
+[@CInline]
+let to_jacob_point p res =
+  let px = getx res in
+  let py = gety res in
+  let pz = getz res in
+  copy px (sub p 0ul 4ul);
+  copy py (sub p 4ul 4ul);
+  bn_set_one4 pz
+
+
+///  Check if a point is on the curve
 
 let lemmaEraseToDomainFromDomain z =
   lemma_mod_mul_distr_l (z * z) z S.prime
@@ -184,86 +224,6 @@ val lemma_norm_as_specification: xD: nat{xD < S.prime} -> yD: nat{yD < S.prime} 
 let lemma_norm_as_specification xD yD zD x3 y3 z3 =
   power_distributivity (zD * zD * zD) (S.prime - 2) S.prime;
   power_distributivity (zD * zD) (S.prime -2) S.prime
-
-
-let norm p resultPoint tempBuffer =
-  let xf = sub p (size 0) (size 4) in
-  let yf = sub p (size 4) (size 4) in
-  let zf = sub p (size 8) (size 4) in
-
-
-  let z2f = sub tempBuffer (size 4) (size 4) in
-  let z3f = sub tempBuffer (size 8) (size 4) in
-  let tempBuffer20 = sub tempBuffer (size 12) (size 20) in
-
-    let h0 = ST.get() in
-  fsqr zf z2f;
-    let h1 = ST.get() in
-  fmul z2f zf z3f;
-    let h2 = ST.get() in
-      lemma_mod_mul_distr_l (fromDomain_ (as_nat h0 zf) * fromDomain_ (as_nat h0 zf)) (fromDomain_ (as_nat h0 zf)) S.prime;
-      assert (as_nat h1 z2f = toDomain_ (fromDomain_ (as_nat h0 zf) * fromDomain_ (as_nat h0 zf) % S.prime));
-      assert (as_nat h2 z3f = toDomain_ (fromDomain_ (as_nat h0 zf) * fromDomain_ (as_nat h0 zf) * fromDomain_ (as_nat h0 zf) % S.prime));
-
-  finv z2f z2f;
-    let h3 = ST.get() in
-      assert(as_nat h3 z2f = toDomain_ (S.pow (fromDomain_ (as_nat h2 z2f)) (S.prime - 2) % S.prime));
-  finv z3f z3f;
-    let h4 = ST.get() in
-      assert(as_nat h4 z3f = toDomain_ (S.pow (fromDomain_ (as_nat h3 z3f)) (S.prime - 2) % S.prime));
-
-  fmul xf z2f z2f;
-  fmul yf z3f z3f;
-  normalisation_update z2f z3f p resultPoint;
-
-    let h3 = ST.get() in
-    lemmaEraseToDomainFromDomain (fromDomain_ (as_nat h0 zf));
-    power_distributivity (fromDomain_ (as_nat h0 zf) * fromDomain_ (as_nat h0 zf)) (S.prime -2) S.prime;
-    Math.Lemmas.nat_times_nat_is_nat (fromDomain_ (as_nat h0 zf)) (fromDomain_ (as_nat h0 zf));
-    Math.Lemmas.nat_times_nat_is_nat (fromDomain_ (as_nat h0 zf) * fromDomain_ (as_nat h0 zf)) (fromDomain_ (as_nat h0 zf));
-    power_distributivity (fromDomain_ (as_nat h0 zf) * fromDomain_ (as_nat h0 zf) * fromDomain_ (as_nat h0 zf)) (S.prime -2) S.prime;
-
-    lemma_norm_as_specification (fromDomain_ (point_x_as_nat h0 p)) (fromDomain_ (point_y_as_nat h0 p)) (fromDomain_ (point_z_as_nat h0 p)) (point_x_as_nat h3 resultPoint) (point_y_as_nat h3 resultPoint) (point_z_as_nat h3 resultPoint);
-
-    assert(
-       let zD = fromDomain_(point_z_as_nat h0 p) in
-       let xD = fromDomain_(point_x_as_nat h0 p) in
-       let yD = fromDomain_(point_y_as_nat h0 p) in
-       let (xN, yN, zN) = S.norm_jacob_point (xD, yD, zD) in
-       point_x_as_nat h3 resultPoint == xN /\ point_y_as_nat h3 resultPoint == yN /\ point_z_as_nat h3 resultPoint == zN)
-
-
-let normX p result tempBuffer =
-  let xf = sub p (size 0) (size 4) in
-  let yf = sub p (size 4) (size 4) in
-  let zf = sub p (size 8) (size 4) in
-
-
-  let z2f = sub tempBuffer (size 4) (size 4) in
-  let z3f = sub tempBuffer (size 8) (size 4) in
-  let tempBuffer20 = sub tempBuffer (size 12) (size 20) in
-
-    let h0 = ST.get() in
-  fsqr zf z2f;
-  finv z2f z2f;
-  fmul z2f xf z2f;
-  fromDomain z2f result;
-  assert_norm (S.prime >= 2);
-    power_distributivity (fromDomain_ (as_nat h0 zf) * fromDomain_ (as_nat h0 zf)) (S.prime -2) S.prime
-
-
-
-#push-options "--ifuel 1"
-
-let bufferToJac p result =
-  let partPoint = sub result (size 0) (size 8) in
-  copy partPoint p;
-  upd result (size 8) (u64 1);
-  upd result (size 9) (u64 0);
-  upd result (size 10) (u64 0);
-  upd result (size 11) (u64 0)
-
-#pop-options
 
 
 inline_for_extraction noextract
@@ -405,7 +365,7 @@ let verifyQ pubKey =
       SD.changeEndianLemma (BSeq.uints_from_bytes_be (as_seq h1 (gsub pubKey (size 32) (size 32))));
       BSeq.uints_from_bytes_be_nat_lemma #U64 #_ #4 (as_seq h1 (gsub pubKey (size 32) (size 32)));
 
-  bufferToJac publicKeyB publicKeyJ;
+  to_jacob_point publicKeyB publicKeyJ;
   let r = verifyQValidCurvePoint publicKeyJ in
   pop_frame();
   r
